moving combinators for wp and req ens commutation to prims

ulib/prims.fst
@@ -249,8 +249,18 @@ new_effect GHOST = PURE
 unfold
 let purewp_id (a:Type) (wp:pure_wp a) = wp
 
-sub_effect
-  PURE ~> GHOST = purewp_id
+unfold
+let weaken_pure_wp (a:Type) (wp:pure_wp a) (p:Type0) =
+  fun post -> p ==> wp post
+
+unfold
+let strengthen_pure_wp (a:Type) (wp:pure_wp a) (p:Type0) =
+  fun post -> p /\ wp post
+
+unfold
+let trivial_pure_post (a:Type) : pure_post a = fun _ -> True
+
+sub_effect PURE ~> GHOST = purewp_id
 
 (* The primitive effect GTot is definitionally equal to an instance of GHOST *)
 effect GTot (a:Type) = GHOST a (pure_null_wp a)
@@ -479,3 +489,75 @@ let labeled (r:range) (msg:string) (b:Type) :Type = b
 private
 abstract
 let __cache_version_number__ = 16
+
+
+
+
+[@"opaque_to_smt"]
+let as_requires_opaque (#a:Type) (wp:pure_wp a) = as_requires wp
+[@"opaque_to_smt"]
+let as_ensures_opaque (#a:Type) (wp:pure_wp a) = as_ensures wp
+
+private irreducible let wp_req_ens_attr : Type0 = True
+
+[@wp_req_ens_attr "opaque_to_smt"]
+private let as_requires_return (a:Type) (x:a) : pure_pre = True
+
+[@wp_req_ens_attr "opaque_to_smt"]
+private let as_ensures_return (a:Type) (x:a) : pure_post a = fun r -> r == x
+
+[@wp_req_ens_attr "opaque_to_smt"]
+private let as_requires_bind (a:Type) (b:Type) (wp1:pure_wp a) (wp2:a -> GTot (pure_wp b))
+: pure_pre
+= as_requires_opaque wp1 /\ (forall (x:a). (as_ensures_opaque wp1) x ==> as_requires_opaque (wp2 x))
+
+[@wp_req_ens_attr "opaque_to_smt"]
+private let as_ensures_bind (a:Type) (b:Type) (wp1:pure_wp a) (wp2:a -> GTot (pure_wp b))
+: pure_post b
+= fun (y:b) -> exists (x:a). (as_ensures_opaque wp1) x /\ (as_ensures_opaque (wp2 x)) y
+
+[@wp_req_ens_attr "opaque_to_smt"]
+private let as_requires_weaken (a:Type) (wp:pure_wp a) (p:Type0) : pure_pre
+= p ==> as_requires_opaque wp
+
+[@wp_req_ens_attr "opaque_to_smt"]
+private let as_ensures_weaken (a:Type) (wp:pure_wp a) (_:Type0) : pure_post a
+= as_ensures_opaque wp
+
+[@wp_req_ens_attr "opaque_to_smt"]
+private let as_requires_strengthen (a:Type) (wp:pure_wp a) (p:Type0) : pure_pre
+= p /\ as_requires_opaque wp
+
+[@wp_req_ens_attr "opaque_to_smt"]
+private let as_ensures_strengthen (a:Type) (wp:pure_wp a) (_:Type0) : pure_post a
+= as_ensures_opaque wp
+
+[@wp_req_ens_attr "opaque_to_smt"]
+private let as_requires_if_then_else (a:Type) (p:Type0) (wp_then:pure_wp a) (wp_else:pure_wp a)
+: pure_pre
+= (p ==> as_requires_opaque wp_then) /\ ((~ p) ==> as_requires_opaque wp_else)
+
+[@wp_req_ens_attr "opaque_to_smt"]
+private let as_ensures_if_then_else (a:Type) (p:Type0) (wp_then:pure_wp a) (wp_else:pure_wp a)
+: pure_post a
+= fun (x:a) -> (p ==> (as_ensures_opaque wp_then) x) /\ ((~ p) ==> (as_ensures_opaque wp_else) x)
+
+[@wp_req_ens_attr "opaque_to_smt"]
+private let as_requires_ite (a:Type) (wp:pure_wp a) : pure_pre = as_requires_opaque wp
+
+[@wp_req_ens_attr "opaque_to_smt"]
+private let as_ensures_ite (a:Type) (wp:pure_wp a) : pure_post a = as_ensures_opaque wp
+
+[@wp_req_ens_attr "opaque_to_smt"]
+private let as_requires_close (a:Type) (b:Type) (wp:b -> GTot (pure_wp a)) : pure_pre
+= forall (b:b). as_requires_opaque (wp b)
+
+[@wp_req_ens_attr "opaque_to_smt"]
+private let as_ensures_close (a:Type) (b:Type) (wp:b -> GTot (pure_wp a)) : pure_post a
+= fun (x:a) -> forall (b:b). as_ensures_opaque (wp b) x
+
+[@wp_req_ens_attr "opaque_to_smt"]
+private let as_requires_null (a:Type) : pure_pre = True
+
+[@wp_req_ens_attr "opaque_to_smt"]
+private let as_ensures_null (a:Type) : pure_post a = fun _ -> True
